---
layout:      post
title:       "Exercise 2.14: Concentration Around Medians and Means"
sorting_tag: "214"
tags:        [chapter 2, layer cake, symmetrisation, Chernoff bound, incomplete]
comments:    true
date:        2020-08-25
---

## (a)

By the layer cake trick
\begin{align}
  \V (X)
  =
  \int_0^\infty
    \P ((X - \mu)^2 > t)
    \, \sd t
  \leq
  c_1
  \int_0^\infty
    e^{- c_2 t}
    \, \sd t
  =
  \frac{c_1}{c_2}
  \, .
\end{align}


## (b)

Take $$ X $$ to be a Rademacher random variable. Then any $$ m_X \in [-1 , 1] $$
is a median.


## (c)

We will proceed by proving the bound for the case of (i) large
$$ t \geq \alpha \Delta $$, and (ii) small $$ t < \alpha \Delta $$, where
$$ \Delta = | \E [X] - m_X |$$, and
$$ \alpha > 0 $$ is an auxiliary parameter which we will choose later.

__(i) $$ t \geq \alpha \Delta $$:__
Using $$ | X - m_X | \leq \Delta + | X - E [X] | $$
\begin{align}
  \P (|X - m_X| \geq t)
  &=
  \P \left(|X - m_X| \geq \tfrac{t}{\alpha} + (1 - \tfrac{1}{\alpha})t\right)
  \newline
  &\leq
  \P \left( | X - m_X | \geq \Delta + (1 - \tfrac{1}{\alpha}) t \right)
  \newline
  &\leq
  \P \left( | X - \E [X] | \geq (1 - \tfrac{1}{\alpha}) t \right)
  \leq
  c_1 e^{-c_2 (1 - \alpha^{-1})^2 t^2}
  \, .
\end{align}

__(ii) $$ t < \alpha \Delta $$:__ Noticing the bound from (i) grows
as $$ t \downarrow 0 $$, the strategy we take is to inflate said bound
sufficiently so that it holds vacuously for all $$ 0 \leq t < \alpha \Delta $$.
Introducing another auxiliary parameter $$ \beta \geq 1 $$, we therefore require
\begin{align}
  \beta c_1 e^{-c_2 (1 - \alpha^{-1})^2 t^2}
  \>
  \beta c_1 e^{-c_2 (\alpha - 1)^2 \Delta^2}
  \geq
  1
  \geq
  \P (|X - m_X| \geq t)
  \, .
\end{align}
The crucial observation here is that the assumed bounds
\begin{align}
  \P (X \geq \E [X] + t) &\leq c_1 e^{- c_2 t^2 } \, , \newline
  \P (X \leq \E [X] - t) &\leq c_1 e^{- c_2 t^2 } \, ,
\end{align}
imply that for either $$ \E [X] + t $$ or $$ \E [X] - t $$ to be a median
(i.e., satisfy $$ \P (X \geq m_X) \geq \tfrac{1}{2} $$ and
$$ \P (X \leq m_X) \geq \tfrac{1}{2} $$ respectively),
we must have $$ c_1 e^{- c_2 t^2 } \geq \frac{1}{2} $$.
Hence
\begin{align}
  m_X
  \in
  \left[
    \E[X] - \sqrt{\tfrac{1}{c_2}\log(2 c_1)} ,
    \E[X] + \sqrt{\tfrac{1}{c_2}\log(2 c_1)}
  \right]
  \, ,
\end{align}
which provides a bound for $$ \Delta $$.
Substituting into the above expression
\begin{align}
  \beta c_1 e^{- c_2 (\alpha - 1)^2 \Delta^2}
  \geq
  \beta c_1 e^{- (\alpha - 1)^2 \log 2 c_1}
  =
  \beta c_1 \left( \tfrac{1}{2 c_1} \right)^{(\alpha - 1)^2}
  \geq
  1
  \, .
\end{align}
Since we have no control over $$ c_1 $$, we must set
$$ \alpha = 2 $$ ($$ \alpha = 0 $$ is inadmissable because we have divided by
$$ \alpha $$ above). This then also necessitates setting $$ \beta = 2 $$.

Putting (i) and (ii) together
\begin{align}
  \P (|X - m_X| \geq t)
  \leq
  c_3
  e^{- c_4 t^2}
  \, ,
\end{align}
for $$ c_3 = 2 c_1 $$ and $$ c_4 = \tfrac{c_2}{4} $$ which improves upon
each of the required constants by a factor of two.

## (c) Alternative Solution

Suppose that we have concentration around some value $$a$$:
\begin{equation}
    \P(\abs{X - a} \ge t) \le c_1 e^{-c_2 t^2}.
\end{equation}
We aim for concentration around another value $$b$$.
Let $$\Delta = \abs{a - b}$$ be the difference between the two values.
The key insight is that a far enough deviation from $$b$$ implies a deviation from $$a$$:
\begin{equation}
    \P(\abs{X - b} \ge t) \le \P(\abs{X - a} \ge \tfrac12 t) \le c_1 e^{-\frac14 c_2 t^2} = f(t)
\end{equation}
for $$t \ge 2 \Delta$$.
For $$t \le 2 \Delta$$, we have the trivial bound
\begin{equation}
    \P(\abs{X - b} \ge t) \le 1.
\end{equation}
To unify these two bounds into one, we require that
\begin{equation}
    \inf_{t \in [0, 2 \Delta]} f(t) = f(2 \Delta) = c_1 e^{-c_2 \Delta^2} \ge 1.
\end{equation}
Then, for all $$t \ge 0$$, we have
\begin{equation}
    \P(\abs{X - b} \ge t)
    \le \parens{1 \lor \frac{1}{c_1} e^{c_2 \Delta^2}} c_1 e^{-\frac14 c_2 t^2}
    \le \parens{c_1 \lor e^{c_2 \Delta^2}} e^{-\frac14 c_2 t^2}.
\end{equation}

Let $$b$$ be a median.
We can develop an upper bound on $$\Delta$$.
Note that
\begin{equation}
    \P(X \ge a + t) \le c_1 e^{-c_2 t^2}.
\end{equation}
If the RHS is strictly less than $$\frac12$$, then $$\P(X \ge a + t) < \tfrac12$$, so $$a + t$$ cannot be a median.
In particular, it must be greater than all medians, so
\begin{equation}
    a + t \ge b \implies b - a \le t.
\end{equation}
Similarly, note that
\begin{equation}
    \P(X \le a - t) \le c_1 e^{-c_2 t^2}.
\end{equation}
Again, if the RHS is strictly less than $$\frac12$$, then $$\P(X \le a - t) < \tfrac12$$, so $$a - t$$ cannot be a median.
In particular, it must be smaller than all medians, so
\begin{equation}
    a - t \le b \implies a - b \le t.
\end{equation}
In conclusion, $$\Delta = \abs{a - b} \le t$$ for all $$t$$ such that
\begin{equation}
    c_1 e^{-c_2 t^2} = \alpha
    \implies
    t = \sqrt{\log(c_1/\alpha)/c_2}
\end{equation}
with $$\alpha \in (0, \frac12)$$.
Then take $$\alpha \uparrow \frac12$$ to find that
\begin{equation}
    \Delta \le \sqrt{\log(2 c_1)/c_2}.
\end{equation}
With this upper bound, we have
\begin{equation}
    \P(\abs{X - b} \ge t) \le 2 c_1 e^{-\frac14 c_2 t^2}.
\end{equation}

Alternatively, a lower bound on $$f(2 \Delta)$$ can be obtained.
Note that
\begin{equation}
    f(2 \Delta)
    \ge \P(\abs{X - a} \ge \Delta).
\end{equation}
If $$a \le b$$, then
\begin{equation}
    \P(X \ge b) \le \P(\abs{X - a} \ge \Delta).
\end{equation}
If $$a \ge b$$, then
\begin{equation}
    \P(X \le b) \le \P(\abs{X - a} \ge \Delta).
\end{equation}
Hence,
\begin{equation}
    f(2 \Delta) \ge \P(X \ge b) \land \P(X \le b).
\end{equation}
Therefore,
\begin{equation}
    \P(\abs{X - b} \ge t)
    \le \frac{c_1}{\P(X \ge b) \land \P(X \le b)}  e^{-\frac14 c_2 t^2}.
\end{equation}
If $$b$$ is a median, then
\begin{equation}
    \P(\abs{X - b} \ge t)
    \le 2 c_1 e^{-\frac14 c_2 t^2}.
\end{equation}
More generally, if $$b$$ is an $$\alpha$$-quantile with $$\alpha \in (0, \tfrac12]$$, then
\begin{equation}
    \P(\abs{X - b} \ge t)
    \le \frac{c_1}{\alpha} e^{-\frac14 c_2 t^2}.
\end{equation}
Note that the results hold for *any* $$a$$.

## (d)

Let us start off by combining the Chernoff bound with the inequality
$$ e^{\lambda |x|} \leq e^{\lambda x} + e^{-\lambda x} $$
\begin{align}
  \P (| X - \E [X] | \geq t)
  &\leq
  \inf\_{\lambda > 0}
    \frac{
      \E [e^{\lambda (X - \E[X])}]
      +
      \E [e^{-\lambda (X - \E[X])}]
    }{e^{\lambda t}}
  \, .
\end{align}
Introducing $$ Y $$, an independent copy of $$ X $$, we use the Jensen's
inequality to bound
\begin{align}
  \E_X [e^{\lambda (X - \E_Y[Y])}]
  \leq
  \E_{X, Y} [e^{\lambda (X - Y)}]
  \, .
\end{align}
Assuming integrability (which we prove momentarily), we can expand
\begin{align}\label{eq:d_mgf_bound}
  \E [e^{\lambda (X - Y)}]
  =
  1
  +
  \sum\_{n = 1}^{\infty}
    \frac{\lambda^n}{n!}
    \E [(X - Y)^n]
  \, .
\end{align}
Observing $$ X - Y $$ is symmetric, it is clear that every finite _odd_ moment
vanishes. This then allows restricting our attention to bounding the _even_
moments, which can be done using the layer cake trick
\begin{align}
  \E [|X - Y|^n]
  &=
  \int\_0^\infty
    \P (|X - Y|^n \geq u) \, \sd u
  \newline
  &\overset{\text{(i)}}{\leq}
  n \int\_0^\infty v^{n - 1} \P (|X - Y| \geq v) \, \sd v
  \newline
  &\overset{\text{(ii)}}{\leq}
  2n \int\_0^\infty v^{n - 1} \P (|X - m\_X| \geq \tfrac{v}{2}) \, \sd v
  \, ,
\end{align}
where (i) follows by the change of variable $$ u = v^n $$, and (ii) uses
the triangle inequality $$ | X - Y | \leq | X - m_x | + | Y - m_X | $$ in
combination with $$ X $$ and $$ Y $$ being i.i.d.
\begin{align}
 \P (| X - Y | < t)
 \geq
 \P ( | X - m\_X | < \tfrac{t}{2} )
 \P ( | Y - m\_X | < \tfrac{t}{2} )
 \, ,
\end{align}
which after taking complements and rearranging yields
\begin{align}\label{eq:d_symmetrised_deviation_bound}
 \P (| X - Y | \geq t)
 \leq
 2 \P (|X - m\_X| \geq \tfrac{t}{2})
 -
 \P (|X - m\_X| \geq \tfrac{t}{2})^2
 \leq
 2 \P (|X - m\_X| \geq \tfrac{t}{2})
 \, .
\end{align}

Substituting the assumed
$$ P(|X - m_X| \geq \tfrac{v}{2}) \leq c_3 e^{-c_4 t^2} $$
\begin{align}
  \E [|X - Y|^n]
  &\leq
  2n c\_3 \int\_0^\infty v^{n - 1} e^{- c\_4 \frac{v^2}{4}}
  \frac{
    \sqrt{2\pi \cdot 2 / c\_4}
  }{
    \sqrt{2\pi \cdot 2 / c\_4}
  }
  \, \sd v
  \newline
  &=
  2 n c\_3 \sqrt{\frac{\pi}{c\_4}}
  \int\_{-\infty}^{\infty}
    |v|^{n - 1}
    \frac{
      e^{- \frac{c\_4}{4} v^2}
    }{
      \sqrt{2\pi \cdot 2 / c\_4}
    }
    \, \sd v
  \newline
  &=
  c\_3 n
  \bigl( \tfrac{2}{\sqrt{c\_4}} \bigr)^{n}
  \Gamma \bigl( \tfrac{n}{2} \bigr)
  \, ,
\end{align}
where the last equality uses the
[closed-form expression](https://en.wikipedia.org/wiki/Normal_distribution#Moments)
for absolute moment of a centred Gaussian variable
$$ Z \sim \gauss (0, \tfrac{2}{c_4}) $$
\begin{align}
  \E [|Z|^{n - 1}]
  =
  \biggl( \frac{2}{c\_4} \biggr)^{\frac{n - 1}{2}}
  \frac{
    2^{\frac{n - 1}{2}} \Gamma\bigl(\tfrac{n}{2}\bigr)
  }{\sqrt{\pi}}
\end{align}
with $$ \Gamma $$ standing for the
[Gamma function](https://en.wikipedia.org/wiki/Gamma_function).
Substituting the bound for the even moments into Equation \eqref{eq:d_mgf_bound}
\begin{align}
  \E [e^{\lambda(X - Y)}]
  &=
  1
  +
  \sum\_{k = 1}^{\infty}
    \frac{\lambda^{2k}}{(2k)!}
    \E [ | X - Y |^{2k} ]
  \newline
  &\overset{\text{(i)}}{\leq}
  1
  +
  c\_3
  \sum\_{k = 1}^{\infty}
    \biggl( \frac{2\lambda}{\sqrt{c\_4}} \biggr)^{2k}
    \frac{\Gamma(k)}{\Gamma (2k)}
  \newline
  &\overset{\text{(ii)}}{\leq}
  1
  +
  c\_3
  \sum\_{k = 1}^\infty
    \biggl( \frac{4 \lambda^2}{c\_4} \biggr)^k
    \frac{1}{k!}
  \newline
  &\overset{\text{(iii)}}{\leq}
  c\_3 e^{\frac{4 \lambda^2}{c\_4}}
  \, ,
\end{align}
where (i) uses the identity $$ \Gamma (2k) = (2k - 1)! $$, (ii) follows by
the same identity and $$ \frac{1}{(2k - 1) \cdots k} \leq \frac{1}{k!} $$, and
(iii) exploits $$ c_3 \geq 1 $$: since the bound
$$ P(|X - m_X| \geq t) \leq c_3 e^{-c_4 t^2} $$ holds for all $$ t \geq 0 $$,
taking $$ t \downarrow 0 $$ reveals $$ c_3 \geq 1 $$.

Because the same argument can be applied to bound
$$ \E [e^{-\lambda (X - \E [X])}]$$, we can substitute into our Chernoff bound
\begin{align}
  \P (|X - \E [X]| \geq t)
  &\leq
  2 c\_3 \inf_{\lambda > 0}
    e^{\frac{4 \lambda^2}{c\_4} - \lambda t}
  =
  c\_1 e^{- c\_2 t^2}
  \, ,
\end{align}
with $$ c_1 = 2 c_3 $$ and $$ c_2 = \frac{c_4}{8} $$.

<span class="accent">
   This bound is valid but **does not match the required $$c_2$$ constant!**
</span>

## (d) Alternative Solution Using the Layer Cake Trick Directly

Applying the Chernoff bound, for any $$ \lambda > 0 $$
\begin{align}
  \P ( | X - \E [X] | \geq t )
  =
  \P \bigl( e^{\lambda (X - \E [X])^2} \geq e^{\lambda t^2} \bigr)
  \leq
  e^{- \lambda t^2}
  \E \bigl[e^{\lambda (X - \E [X])^2}\bigr]
  \, .
\end{align}
Since we are trying to establish $$ X - \E [X] $$ behaves like a sub-Gaussian
random variable, and Theorem 2.6(IV) tells that sub-Gaussianity implies
$$ \E [ e^{\lambda (X - \E[X])^2} ] < \infty $$, our goal will be to obtain
a similar bound here.

Introducing $$ Y $$, an independent copy of $$ X $$, the Jensen's inequality can
be applied to the convex function $$ x \mapsto e^{\lambda x^2} $$ to obtain the
symmetrised
\begin{align}
  \E_X \bigl[e^{\lambda (X - \E_Y [Y])^2}\bigr]
  \leq
  \E_{X, Y} \bigl[e^{\lambda (X - Y)^2}\bigr]
  \, .
\end{align}
The right-hand side can be bounded using the layer cake trick
\begin{align}
  \E \bigl[ e^{\lambda (X - Y)^2} \bigr]
  &=
  \int\_0^\infty
    \P \bigl( e^{\lambda (X - Y)^2} \geq u \bigr) \, \sd u
  \newline
  &\overset{\text{(i)}}{\leq}
  \alpha
  +
  \int\_{\alpha}^\infty
    \P \bigl( e^{\lambda (X - Y)^2} \geq u \bigr) \, \sd u
  \newline
  &\overset{\text{(ii)}}{=}
  \alpha
  +
  \lambda
  \int\_{\frac{\log \alpha}{\lambda}}^\infty
    e^{\lambda v}
    \P (|X - Y| \geq \sqrt{v})
    \, \sd v
  \, ,
\end{align}
where (i) introduces a parameter $$ \alpha \geq 1 $$ which we will optimise
later, and (ii) follows by substituting $$ u = e^{\lambda v} $$.
Using the bound from Equation \eqref{eq:d_symmetrised_deviation_bound} to bound
the second term
\begin{align}
  \lambda
  \int\_{\frac{\log \alpha}{\lambda}}^\infty
    e^{\lambda v}
    \P (|X - Y| \geq \sqrt{v})
    \, \sd v
  &\leq
  2 \lambda
  \int\_{\frac{\log \alpha}{\lambda}}^\infty
    e^{\lambda v}
    \P (|X - m_x| \geq \tfrac{\sqrt{v}}{2})
    \, \sd v
  \newline
  &\overset{\text{(i)}}{\leq}
  2 \lambda c\_3
  \int\_{\frac{\log \alpha}{\lambda}}^\infty
    e^{(\lambda - \frac{c\_4}{4}) v}
    \, \sd v
  \newline
  &=
  2 \lambda c\_3
  \biggl[
    \frac{e^{(\lambda - \frac{c\_4}{4}) v}}{\lambda - \frac{c\_4}{4}}
  \biggr]\_{\frac{\log \alpha}{\lambda}}^\infty
  \overset{\text{(ii)}}{=}
  \frac{8 \lambda c\_3}{c\_4 - 4\lambda}
  \alpha^{-\left(\frac{c\_4}{4 \lambda} - 1 \right)}
\end{align}
where (i) is by substitution of the assumed concentration bound around the
median, and (ii) holds whenever $$ \lambda < \frac{c_4}{4} $$.
Substituting into our bound for $$ \E [e^{\lambda (X - Y)^2}] $$
\begin{align}
   \E \bigl[e^{\lambda (X - Y)^2}\bigr]
   &\leq
   \alpha \left(
     1
     +
     c
     \alpha^{-p}
   \right)
   \, ,
\end{align}
where we defined $$ c = \frac{8 \lambda c_3}{c_4 - 4\lambda} $$ and
$$ p = \frac{c_4}{4 \lambda} $$.

We are now in position to optimise over $$ \alpha \geq 1 $$.
Setting the derivative to zero, the unconstrained optimum is
$$ \alpha = [c (p - 1)]^{1 / p} = (2 c_3)^{1 / p} $$.
Since $$ c_3 \geq 1 $$ (see above), $$ \alpha = (2 c_3)^{1 / p} $$
is also the constrained optimum.
Substituting
\begin{align}
   \E \bigl[e^{\lambda (X - Y)^2}\bigr]
   &\leq
   [
     c (p - 1)
   ]^{1/p}
   +
   c
   =
   (2 c\_3)^{\frac{4 \lambda}{c_4}}
   +
   \frac{8 \lambda c_3}{c_4 - 4\lambda}
   \, .
\end{align}

The only remaining task is to optimise over $$ \lambda < \frac{c_4}{4} $$
\begin{align}
  \P (|X - \E [X]| \geq t)
  \leq
  e^{-\lambda t^2}
  \left[
    (2 c\_3)^{\frac{4 \lambda}{c_4}}
    +
    \frac{8 \lambda c_3}{c_4 - 4\lambda}
  \right]
  \, .
\end{align}
Making $$ \lambda $$ too small would yield the vacuous unit bound, while
approaching $$ \frac{c_4}{4} $$ from below makes the second term explode.
We thus somewhat arbitrarily take the midpoint $$ \lambda = \frac{c_4}{8} $$
which results in
\begin{align}
  \P (|X - \E [X]| \geq t)
  \leq
  c\_1
  e^{- c\_2 t^2 }
  \, ,
\end{align}
with $$ c_1 = \sqrt{2 c_3} (1 + \sqrt{2 c_3}) $$ and
$$ c_2 = \frac{c_4}{8} $$.

<span class="accent">
   The above bound is valid but **does not match the required constants!**
</span>


## Notes

- There is nothing special about the median in (d). In fact, we can obtain
a concentration bound for the mean similar to (d), whenever there exists
$$ a \in \R $$ such that $$ \P ( |X - a| \geq t ) \leq c_3 e^{-c_4 t^2} $$.
