---
layout:      post
title:       "Exercise 5.11: Details of Example 5.19"
sorting_tag: "0511"
tags:        [chapter 5,incomplete]
comments:    true
---

## (a)
The inequality follows directly from the Von Neumann trace inequality, and note that $\norm{W}_2$ is achieved by setting $\Theta$ equal to the outer product of the right and left singular vectors of $W$ corresponding to the largest singular value.

## (b)
Simply note that
\begin{equation}
    X_\Theta - X_{\Theta'}
    = \lra{W, \Theta - \Theta'}
    \in \SG(\norm{\Theta - \Theta'}_F),
\end{equation}
using that the entries of $W$ are independent and in $\SG(1)$.

## (c)
By the Von Neumann trace inequality and using that $\rank(\Sigma - \Sigma') \le 2$,
\begin{equation}
    \lra{\Gamma - \Gamma', W}
    \le (\sigma_1(\Gamma - \Gamma') + \sigma_2(\Gamma - \Gamma'))\sigma_1(W)
    \le \sqrt{2} (\sigma_1^2(\Gamma - \Gamma') + \sigma_2^2(\Gamma - \Gamma'))^{\frac12} \sigma_1(W).
\end{equation}
Therefore,
\begin{equation}
    \lra{\Gamma - \Gamma', W}
    \le \sqrt{2}\norm{\Gamma - \Gamma'}_F \norm{W}_2
    \le \sqrt{2} \delta \norm{W}_2.
\end{equation}

## (d)
Consider $ab^\T$ and $xy^\T$ such that $\norm{a b^\T}_F, \norm{x y^\T}_F \le 1$.
Noting that $\norm{a b^\T}_F = \norm{a}\norm{b}$,
without loss of generality, assume that $\norm{a}  = \norm{y} = 1$ and $\norm{b},\norm{x}\le 1$.
Decompose
\begin{align}
    (a_i b_j - x_i y_j)^2
    &= (a_i b_j - a_i y_j + a_i y_j - x_i y_j)^2 \newline
    &= a_i^2 (b_j - y_j)^2 + (a_i - x_i)^2 y_j^2 + 2(a_i^2 - a_i x_i)(b_j y_j - y_j^2).
\end{align}
Then, summing over $i \in [n]$ and $j \in [d]$ and using that $\norm{a}  = \norm{y} = 1$,
\begin{equation}
    \norm{ab^\T - xy^\T}_F^2
    = \norm{b - y}^2 + \norm{a - x}^2 - 2\parens{1 - \lra{a, x}}\parens{1 - \lra{b, y}}
    \le \norm{b - y}^2 + \norm{a - x}^2,
\end{equation}
since $\lra{a, x} \le \norm{x} \le 1$ and similarly $\lra{b, y} \le 1$.
Therefore,
\begin{equation}
    \norm{ab^\T - xy^\T}_F \le \norm{(a, b) - (x, y)},
\end{equation}
which means that the covering is reduced to a covering of the $\sqrt{2}$-ball of $\R^{n + d}$ ($\norm{(a, b)}^2 = \norm{a}^2 + \norm{b}^2 \leq 2$).

<span class="accent">
   This bound is valid but **larger by a $\sqrt{2}$** than what is required!
</span>

## (d) Alternative Solution

We use the equivalent form of the Frobenius norm,
$\norm{A}_F^2 = \sum_i \sigma_i^2(A)$, where $\sigma_i(A)$ is the $i^\text{th}$
singular value of $A$.
Square singular values are equal to the eigenvalues of the Gram matrix
\begin{align}
   G
   :=
   (ab^\top - xy^\top)^\top (ab^\top - xy^\top)
   =
   \norm{a}^2 bb^\top
   \+ \norm{x}^2 yy^\top
   \- \langle a, x \rangle (by^\top + yb^\top)
   \, .
\end{align}
The next step is to show that $y - b$ and $y + b$ are (proportional to) the only
two eigenvectors of $G$ associated with non-zero eigenvalues (recall
$\rank(G) \leq 2$).
With a bit of algebra and w.l.o.g. assuming
$\norm{a} = \norm{b} = \norm{x} = \norm{y} = 1$
(since $\norm{ab^\top} = 1$, $\lbrace (ca)(b/c)^\top \rbrace\_{c > 0}$ are all
equivalent representations of $ab^\top$), we obtain
\begin{align}
  G (y - b)
  &=
  (1 + \langle a, x \rangle) (1 - \langle b, y \rangle) (y - b)
  \, ,
  \newline
  G (y + b)
  &=
  (1 - \langle a, x \rangle) (1 + \langle b, y \rangle) (y + b)
  \, .
\end{align}
By the mentioned relation between the eigenvalues and Frobenius norm
\begin{align}
  \norm{ab^\top - xy^\top}_F^2
  =
  (\tfrac{1}{2} \norm{a + x}^2) (\tfrac{1}{2} \norm{b - y}^2)
  +
  (\tfrac{1}{2} \norm{a - x}^2) (\tfrac{1}{2} \norm{b + y}^2)
  \, ,
\end{align}
where used $1 - \langle a, x \rangle = \tfrac{1}{2} \norm{a - x}^2$ by the unit
norm assumption (analogously for the other terms). Another application of the
unit norm yields $\norm{ab^\top - xy^\top}_F \leq \norm{(a,b) - (x, y)}_2$ as
before.

<span class="accent">
   This bound is valid but **larger by a $\sqrt{2}$** than what is required!
</span>
