---
layout:      post
title:       "Exercise 15.3: Properties of the Kullbackâ€“Leibler Divergence"
sorting_tag: "1503"
tags:        [chapter 15]
comments:    true
---

## (a)
Let $\P \ll \Q$.
Then, by Jensen's Inequality,
\begin{equation}
    \KL(\P, \Q)
    = \E\_\P \log \frac{\sd\P}{\sd\Q}
    = \E\_\Q \frac{\sd\P}{\sd\Q} \log \frac{\sd\P}{\sd\Q}
    \ge \E\_\Q\sbrac{\frac{\sd\P}{\sd\Q}} \log \E\_\Q\sbrac{\frac{\sd\P}{\sd\Q}}
    = 0
\end{equation}
with equality if and only if $\frac{\sd\P}{\sd\Q}$ is constant $\Q$-a.s.
Alternatively,
let $A\_1 \cup \cdots \cup A\_n$ be a partition of the probability space.
If $\Q(A\_i) = 0$, then $\P(A\_i) = 0$ by $\P \ll \Q$.
Therefore,
\begin{align}
    \KL(\P, \Q)
    &= \sum\_{i=1}^n \Q(A\_i) \,\E\_\Q \frac{\ind\_{A\_i}}{\Q(A\_i)} \frac{\sd\P}{\sd\Q} \log \frac{\sd\P}{\sd\Q} \newline
    &\ge \sum\_{i=1}^n \Q(A\_i) \,\E\_\Q\sbrac{ \frac{\ind\_{A\_i}}{\Q(A\_i)} \frac{\sd\P}{\sd\Q}} \log \E\_\Q\sbrac{ \frac{\ind\_{A\_i}}{\Q(A\_i)} \frac{\sd\P}{\sd\Q}} \newline
    &\ge \sum\_{i=1}^n \P(A\_i) \,\log \frac{\P(A\_i)}{\Q(A\_i)}.
\end{align}
In particular, if $\P(A) > \Q(A)$ on some measurable set $A$, then $\KL(\P, \Q) > 0$.

## (b)
Let $(\lambda\_i)\_{i=1}^n \in [0, 1]$ sum to one.
WLOG, assume that $\P = \sum\_{i=1}^n \lambda\_i \P\_i \ll \Q$.
Then
\begin{equation}
    \frac{\sd\P}{\sd\Q} = \sum\_{i=1}^n \lambda\_i \frac{\sd\P\_i}{\sd\Q},
\end{equation}
so, using Jensen's Inequality,
\begin{equation}
    \KL(\P, \Q)
    = \E\_\Q \frac{\sd\P}{\sd\Q} \log \frac{\sd\P}{\sd\Q}
    \le \sum\_{i=1}^n \lambda\_i \, \E\_\Q \frac{\sd\P\_i}{\sd\Q} \log \frac{\sd\P\_i}{\sd\Q}.
\end{equation}
Conversely, let $\mu = \tfrac12 (\P + \Q)$.
Then still
\begin{equation}
    \frac{\sd\P}{\sd\mu} = \sum\_{i=1}^n \lambda\_i \frac{\sd\P\_i}{\sd\mu},
\end{equation}
so, by Jensen's Inequality again,
\begin{equation}
    \KL(\Q, \P)
    = -\E\_\Q \log \frac{\sd \P/\sd \mu}{\sd \Q/ \sd \mu}
    \le -\sum\_{i=1}^n \E\_\Q \log  \frac{\sd \P\_i/\sd \mu}{\sd \Q/ \sd \mu}.
\end{equation}

## (c)
Follows directly from the observation that
\begin{equation}
    \frac{\sd(\P\_1 \otimes \P\_2)}{\sd(\Q\_1 \otimes \Q\_2)}
    = \frac{\sd \P\_1}{\sd \Q\_1} \frac{\sd \P\_2}{\sd \Q\_2}.
\end{equation}
